proof/Example_Auction.thy
@@ -12,6 +12,21 @@ definition "auction_rules = {auction_bid_rn, auction_accept_rn}"
 definition "broker_rules  = {broker_reserve_rn}" 
 
 section \<open>Fact definitions\<close>
+
+record Value =
+  item_lot      :: symbol
+  item_desc     :: symbol
+  party_buyer   :: party
+  party_broker  :: party
+  price_amount  :: nat
+  price_limit   :: nat
+  budget_total  :: nat
+  budget_remain :: nat
+
+declare Value.make_def[simp]
+definition [simp]:
+  "value0 = Value.make undefined undefined undefined undefined undefined undefined undefined undefined"
+
 (*
 auction side:
 fact Accept  [lot: Symbol, broker: Party, price: Nat]
@@ -26,115 +41,54 @@ fact Reserve [broker: Party, buyer: Party, lot: Nat, offer: Nat]
 fact Budget  [broker: Party, buyer: Party, budget: Nat]
 *)
 
-(* Boilerplate for fact definitions: these would be a lot cleaner if we used a shallow embedding for the types,
-   but they're all pretty mechanical anyway.
-*)
-definition "mk_AcceptPayload lot broker price = vpair (vlit (lsymbol lot)) (vpair (vlit (lparty broker)) (vlit (lnat price)))"
-fun tk_AcceptPayload where
-  "tk_AcceptPayload (vpair (vlit (lsymbol lot)) (vpair (vlit (lparty broker)) (vlit (lnat price)))) = (lot, broker, price)"
-| "tk_AcceptPayload _ = undefined" 
-
-definition "Accept_lot    =       fst o tk_AcceptPayload o fact_value"
-definition "Accept_broker = fst o snd o tk_AcceptPayload o fact_value"
-definition "Accept_ask    = snd o snd o tk_AcceptPayload o fact_value"
 
 definition "Accept = fact_ctor ''Accept''"
-definition "mk_Accept lot broker price by obs = \<lparr>fact_name = Accept, fact_value = mk_AcceptPayload lot broker price, fact_by = by, fact_obs = obs, fact_rules = auction_rules\<rparr>"
-
-
-definition "mk_ItemPayload lot desc ask = vpair (vlit (lsymbol lot)) (vpair (vlit (lsymbol desc)) (vlit (lnat ask)))"
-fun tk_ItemPayload where
-  "tk_ItemPayload (vpair (vlit (lsymbol lot)) (vpair (vlit (lsymbol desc)) (vlit (lnat ask)))) = (lot, desc, ask)"
-| "tk_ItemPayload _ = undefined" 
-
-definition "Item_lot  =       fst o tk_ItemPayload o fact_value"
-definition "Item_desc = fst o snd o tk_ItemPayload o fact_value"
-definition "Item_ask  = snd o snd o tk_ItemPayload o fact_value"
+definition "mk_Accept lot broker price by obs =
+  \<lparr>fact_name = Accept,
+  fact_value = value0 \<lparr>item_lot := lot, party_broker := broker, price_amount := price\<rparr>,
+  fact_by = by, fact_obs = obs, fact_rules = auction_rules\<rparr>"
 
 definition "Item = fact_ctor ''Item''"
-definition "mk_Item lot desc ask by obs = \<lparr>fact_name = Item, fact_value = mk_ItemPayload lot desc ask, fact_by = by, fact_obs = obs, fact_rules = auction_rules\<rparr>"
-
-
-definition "mk_InvoicePayload broker buyer desc amount = vpair (vlit (lparty broker)) (vpair (vlit (lparty buyer)) (vpair (vlit (lsymbol desc)) (vlit (lnat amount))))"
-fun tk_InvoicePayload where
-  "tk_InvoicePayload (vpair (vlit (lparty broker)) (vpair (vlit (lparty buyer)) (vpair (vlit (lsymbol desc)) (vlit (lnat amount))))) = (broker, buyer, desc, amount)"
-| "tk_InvoicePayload _ = undefined" 
-
-definition "Invoice_broker =             fst o tk_InvoicePayload o fact_value"
-definition "Invoice_buyer  =       fst o snd o tk_InvoicePayload o fact_value"
-definition "Invoice_desc   = fst o snd o snd o tk_InvoicePayload o fact_value"
-definition "Invoice_amount = snd o snd o snd o tk_InvoicePayload o fact_value"
+definition "mk_Item lot desc ask by obs =
+  \<lparr>fact_name = Item,
+  fact_value = value0 \<lparr>item_lot := lot, item_desc := desc, price_amount := ask\<rparr>,
+  fact_by = by, fact_obs = obs, fact_rules = auction_rules\<rparr>"
 
 definition "Invoice = fact_ctor ''Invoice''"
-definition "mk_Invoice broker buyer desc amount by obs = \<lparr>fact_name = Invoice, fact_value = mk_InvoicePayload broker buyer desc amount, fact_by = by, fact_obs = obs, fact_rules = auction_rules\<rparr>"
-
-
-definition "mk_BidPayload lot broker buyer price = vpair (vlit (lsymbol lot)) (vpair (vlit (lparty broker)) (vpair (vlit (lparty buyer)) (vlit (lnat price))))"
-fun tk_BidPayload where
-  "tk_BidPayload (vpair (vlit (lsymbol lot)) (vpair (vlit (lparty broker)) (vpair (vlit (lparty buyer)) (vlit (lnat price))))) = (lot, broker, buyer, price)"
-| "tk_BidPayload _ = undefined" 
-
-definition "Bid_lot    =             fst o tk_BidPayload o fact_value"
-definition "Bid_broker =       fst o snd o tk_BidPayload o fact_value"
-definition "Bid_buyer  = fst o snd o snd o tk_BidPayload o fact_value"
-definition "Bid_price  = snd o snd o snd o tk_BidPayload o fact_value"
+definition "mk_Invoice broker buyer desc amount by obs =
+  \<lparr>fact_name = Invoice,
+  fact_value = value0 \<lparr>party_broker := broker, party_buyer := buyer, item_desc := desc, price_amount := amount\<rparr>,
+  fact_by = by, fact_obs = obs, fact_rules = auction_rules\<rparr>"
 
 definition "Bid = fact_ctor ''Bid''"
-definition "mk_Bid lot broker buyer price by obs = \<lparr>fact_name = Bid, fact_value = mk_BidPayload lot broker buyer price, fact_by = by, fact_obs = obs, fact_rules = auction_rules\<rparr>"
-
-(* Offer has same payload as Bid *)
-definition "mk_OfferPayload = mk_BidPayload"
-definition "tk_OfferPayload = tk_BidPayload"
-definition "Offer_lot    = Bid_lot"
-definition "Offer_broker = Bid_broker"
-definition "Offer_buyer  = Bid_buyer"
-definition "Offer_price  = Bid_price"
+definition "mk_Bid lot broker buyer price by obs =
+  \<lparr>fact_name = Bid,
+  fact_value = value0 \<lparr> item_lot := lot, party_broker := broker, party_buyer := buyer, price_amount := price\<rparr>,
+  fact_by = by, fact_obs = obs, fact_rules = auction_rules\<rparr>"
 
 definition "Offer = fact_ctor ''Offer''"
-definition "mk_Offer lot broker buyer price by obs = \<lparr>fact_name = Offer, fact_value = mk_OfferPayload lot broker buyer price, fact_by = by, fact_obs = obs, fact_rules = auction_rules\<rparr>"
-
-
-definition "mk_OrderPayload broker buyer desc limit budget = vpair (vlit (lparty broker)) (vpair (vlit (lparty buyer)) (vpair (vlit (lsymbol desc)) (vpair (vlit (lnat limit)) (vlit (lnat budget)))))"
-fun tk_OrderPayload where
-  "tk_OrderPayload (vpair (vlit (lparty broker)) (vpair (vlit (lparty buyer)) (vpair (vlit (lsymbol desc)) (vpair (vlit (lnat limit)) (vlit (lnat budget)))))) = (broker, buyer, desc, limit, budget)"
-| "tk_OrderPayload _ = undefined" 
-
-definition "Order_broker =                   fst o tk_OrderPayload o fact_value"
-definition "Order_buyer  =             fst o snd o tk_OrderPayload o fact_value"
-definition "Order_desc   =       fst o snd o snd o tk_OrderPayload o fact_value"
-definition "Order_limit  = fst o snd o snd o snd o tk_OrderPayload o fact_value"
-definition "Order_budget = snd o snd o snd o snd o tk_OrderPayload o fact_value"
+definition "mk_Offer lot broker buyer price by obs =
+  \<lparr>fact_name = Offer,
+  fact_value = value0 \<lparr> item_lot := lot, party_broker := broker, party_buyer := buyer, price_amount := price \<rparr>,
+  fact_by = by, fact_obs = obs, fact_rules = auction_rules\<rparr>"
 
 definition "Order = fact_ctor ''Order''"
-definition "mk_Order broker buyer desc limit budget by obs = \<lparr>fact_name = Order, fact_value = mk_OrderPayload broker buyer desc limit budget, fact_by = by, fact_obs = obs, fact_rules = broker_rules\<rparr>"
-
-
-definition "mk_ReservePayload broker buyer lot amount = vpair (vlit (lparty broker)) (vpair (vlit (lparty buyer)) (vpair (vlit (lsymbol lot)) (vlit (lnat amount))))"
-fun tk_ReservePayload where
-  "tk_ReservePayload (vpair (vlit (lparty broker)) (vpair (vlit (lparty buyer)) (vpair (vlit (lsymbol lot)) (vlit (lnat amount))))) = (broker, buyer, lot, amount)"
-| "tk_ReservePayload _ = undefined" 
-
-definition "Reserve_broker =             fst o tk_ReservePayload o fact_value"
-definition "Reserve_buyer  =       fst o snd o tk_ReservePayload o fact_value"
-definition "Reserve_lot    = fst o snd o snd o tk_ReservePayload o fact_value"
-definition "Reserve_amount = snd o snd o snd o tk_ReservePayload o fact_value"
+definition "mk_Order broker buyer desc limit budget by obs =
+  \<lparr>fact_name = Order,
+  fact_value = value0 \<lparr> party_broker := broker, party_buyer := buyer, item_desc := desc, price_limit := limit, budget_total := budget\<rparr>,
+  fact_by = by, fact_obs = obs, fact_rules = broker_rules\<rparr>"
 
 definition "Reserve = fact_ctor ''Reserve''"
-definition "mk_Reserve broker buyer lot amount by obs = \<lparr>fact_name = Reserve, fact_value = mk_ReservePayload broker buyer lot amount, fact_by = by, fact_obs = obs, fact_rules = broker_rules\<rparr>"
-
-
-definition "mk_BudgetPayload broker buyer budget remain = vpair (vlit (lparty broker)) (vpair (vlit (lparty buyer)) (vpair (vlit (lnat budget)) (vlit (lnat remain))))"
-fun tk_BudgetPayload where
-  "tk_BudgetPayload (vpair (vlit (lparty broker)) (vpair (vlit (lparty buyer)) (vpair (vlit (lnat budget)) (vlit (lnat remain))))) = (broker, buyer, budget, remain)"
-| "tk_BudgetPayload _ = undefined" 
-
-definition "Budget_broker =             fst o tk_BudgetPayload o fact_value"
-definition "Budget_buyer  =       fst o snd o tk_BudgetPayload o fact_value"
-definition "Budget_budget = fst o snd o snd o tk_BudgetPayload o fact_value"
-definition "Budget_remain = snd o snd o snd o tk_BudgetPayload o fact_value"
+definition "mk_Reserve broker buyer lot amount by obs =
+  \<lparr>fact_name = Reserve,
+  fact_value = value0 \<lparr>party_broker := broker, party_buyer := buyer, item_lot := lot, price_amount := amount\<rparr>,
+  fact_by = by, fact_obs = obs, fact_rules = broker_rules\<rparr>"
 
 definition "Budget = fact_ctor ''Budget''"
-definition "mk_Budget broker buyer budget remain by obs = \<lparr>fact_name = Budget, fact_value = mk_BudgetPayload broker buyer budget remain, fact_by = by, fact_obs = obs, fact_rules = broker_rules\<rparr>"
+definition "mk_Budget broker buyer budget remain by obs =
+  \<lparr>fact_name = Budget,
+  fact_value = value0 \<lparr>party_broker := broker, party_buyer := buyer, budget_total := budget, budget_remain := remain\<rparr>,
+  fact_by = by, fact_obs = obs, fact_rules = broker_rules\<rparr>"
 
 (* Fact variables *)
 definition "accept_v  = fact_var ''accept''"
@@ -148,21 +102,25 @@ definition "budget_v  = fact_var ''budget''"
 
 section \<open>Auction bid rule\<close>
 
-definition "match_any_when var factctor when consume auth_f = match var (gather_when factctor when) select_any (consume_weight (\<lambda>h. consume)) (gain_auth auth_f)"
-definition "match_any var factctor consume auth_f = match_any_when var factctor (\<lambda>h. True) consume auth_f"
-definition "match_first_when var factctor when fstby consume auth_f = match var (gather_when factctor when) (select_first fstby) (consume_weight (\<lambda>h. consume)) (gain_auth auth_f)"
+definition [simp]: "match_any_when var factctor when consume auth_f = match var (gather_when factctor when) select_any (consume_weight (\<lambda>h. consume)) (gain_auth auth_f)"
+definition [simp]: "match_any var factctor consume auth_f = match_any_when var factctor (\<lambda>h. True) consume auth_f"
+definition [simp]: "match_first_when var factctor when fstby consume auth_f = match var (gather_when factctor when) (select_first fstby) (consume_weight (\<lambda>h. consume)) (gain_auth auth_f)"
 
-definition
+definition [simp]: "field f h v = f (fact_value (h v))"
+
+
+definition [simp]:
   "auction_bid = rule auction_bid_rn
-  [ match_any bid_v Bid 1 (\<lambda>h. {Bid_buyer (h bid_v), Bid_broker (h bid_v)})
+  [ match_any bid_v Bid 1 (\<lambda>h. {field party_buyer h bid_v, field party_broker h bid_v})
   , match_any_when item_v Item
-        (\<lambda>h. Item_lot (h item_v) = Bid_lot (h bid_v) \<and> Bid_price (h bid_v) < Item_ask (h item_v))
+        (\<lambda>h. field item_lot h item_v = field item_lot h bid_v \<and> field price_amount h bid_v \<le> field price_amount h item_v)
         0
         (\<lambda>h. {party ''Mark''})
   ]
   (\<lambda>h. {#
-    mk_Offer (Item_lot (h item_v)) (Bid_broker (h bid_v)) (Bid_buyer (h bid_v)) (Bid_price (h bid_v))
-          {Bid_buyer (h bid_v), Bid_broker (h bid_v), party ''Mark''}
+    mk_Offer (field item_lot    h item_v) (field party_broker h bid_v)
+             (field party_buyer h bid_v)  (field price_amount h bid_v)
+          {field party_buyer h bid_v, field party_broker h bid_v, party ''Mark''}
           {party ''Mark''}
   #})"
 
@@ -171,69 +129,87 @@ definition
   "auction_accept = rule auction_accept_rn
   [ match_any accept_v Accept 1 (\<lambda>h. {party ''Mark''})
   , match_any_when offer_v Offer
-        (\<lambda>h. Offer_lot (h offer_v) = Accept_lot (h accept_v) \<and> Offer_broker (h offer_v) = Accept_broker (h accept_v))
+        (\<lambda>h. field item_lot h offer_v = field item_lot h accept_v
+           \<and> field party_broker h offer_v = field party_broker h accept_v)
         1
-        (\<lambda>h. {Offer_broker (h offer_v), Offer_buyer (h offer_v)})
+        (\<lambda>h. {field party_broker h offer_v, field party_buyer h offer_v})
   , match_any_when item_v Item
-        (\<lambda>h. Offer_lot (h offer_v) = Item_lot (h item_v))
+        (\<lambda>h. field item_lot h offer_v = field item_lot h item_v)
         1
         (\<lambda>h. {party ''Mark''})
 
   ]
   (\<lambda>h. {#
-    mk_Invoice (Offer_broker (h offer_v)) (Offer_buyer (h offer_v)) (Item_desc (h item_v)) (Offer_price (h offer_v))
-          {Offer_buyer (h offer_v), Offer_broker (h offer_v), party ''Mark''}
+    mk_Invoice (field party_broker h offer_v) (field party_buyer  h offer_v)
+               (field item_desc    h item_v)  (field price_amount h offer_v)
+          {field party_buyer h offer_v, field party_broker h offer_v, party ''Mark''}
           {}
   #})"
 
 
 definition
   "broker_reserve = rule broker_reserve_rn
-  [ match_any order_v Order 0 (\<lambda>h. {Order_buyer (h order_v)})
+  [ match_any order_v Order 0 (\<lambda>h. {field party_buyer h order_v})
   , match_first_when item_v Item
-        (\<lambda>h. Item_desc (h item_v) = Order_desc (h order_v))
-        (\<lambda>h. Item_ask (h item_v))
+        (\<lambda>h. field item_desc    h item_v = field item_desc h order_v)
+        (\<lambda>h. field price_amount h item_v)
         0
         (\<lambda>h. {party ''Mark''})
   , match_any_when reserve_v Reserve
-        (\<lambda>h. Reserve_broker (h reserve_v) = Order_broker (h order_v)
-           \<and> Reserve_buyer  (h reserve_v) = Order_buyer  (h order_v)
-           \<and> Reserve_lot    (h reserve_v) = Item_lot     (h item_v)
-           \<and> Reserve_amount (h reserve_v) \<le> Order_limit  (h order_v))
+        (\<lambda>h. field party_broker h reserve_v = field party_broker h order_v
+           \<and> field party_buyer  h reserve_v = field party_buyer  h order_v
+           \<and> field item_lot     h reserve_v = field item_lot     h item_v
+           \<and> field price_amount h reserve_v \<le> field price_limit  h order_v)
         1
-        (\<lambda>h. {Reserve_broker (h reserve_v)})
+        (\<lambda>h. {field party_broker h reserve_v})
   , match_any_when budget_v Budget
-        (\<lambda>h. Reserve_broker (h reserve_v) = Budget_broker (h budget_v)
-           \<and> Reserve_buyer  (h reserve_v) = Budget_buyer  (h budget_v)
-           \<and> Reserve_amount (h reserve_v) \<le> Budget_remain (h budget_v))
+        (\<lambda>h. field party_broker h reserve_v = field party_broker h budget_v
+           \<and> field party_buyer  h reserve_v = field party_buyer  h budget_v
+           \<and> field price_amount h reserve_v \<le> field budget_remain h budget_v)
         1
-        (\<lambda>h. {Budget_broker (h budget_v)})
+        (\<lambda>h. {field party_broker h budget_v})
   ]
   (\<lambda>h. {#
-    mk_Budget (Budget_broker (h budget_v)) (Budget_buyer (h budget_v)) (Budget_budget (h budget_v))
-          (Budget_remain (h budget_v) - Reserve_amount (h reserve_v))
-          {Budget_broker (h budget_v)}
+    mk_Budget
+          (field party_broker  h budget_v)
+          (field party_buyer   h budget_v)
+          (field budget_total  h budget_v)
+          (field budget_remain h budget_v - field price_amount h reserve_v)
+          {field party_broker  h budget_v}
           {}
-  , mk_Bid (Item_lot (h item_v)) (Reserve_broker (h reserve_v)) (Order_buyer (h order_v)) (Reserve_amount (h reserve_v))
-          {Reserve_broker (h reserve_v), Order_buyer (h order_v)}
+  , mk_Bid
+          (field item_lot     h item_v)
+          (field party_broker h reserve_v)
+          (field party_buyer  h order_v)
+          (field price_amount h reserve_v)
+          {field party_broker h reserve_v, field party_buyer h order_v}
           {party ''Mark''}
   #})"
 
 
 section \<open>Invariants\<close>
 
-definition facts_of_type :: "fact_ctor \<Rightarrow> store \<Rightarrow> store" where
+definition facts_of_type :: "fact_ctor \<Rightarrow> Value store \<Rightarrow> Value store" where
 "facts_of_type ctor s = {# f \<in># s. fact_name f = ctor #}"
 
 definition "bids_for_budget s b =
-  {# f \<in># facts_of_type Bid     s. Bid_buyer     f = Budget_buyer b \<and> Bid_broker     f = Budget_broker b #}"
+  {# f \<in># facts_of_type Bid s.
+    party_buyer  (fact_value f) = party_buyer  (fact_value b)
+  \<and> party_broker (fact_value f) = party_broker (fact_value b) #}"
+
 definition "invoices_for_budget s b =
-  {# f \<in># facts_of_type Invoice s. Invoice_buyer f = Budget_buyer b \<and> Invoice_broker f = Budget_broker b #}"
+  {# f \<in># facts_of_type Invoice s.
+    party_buyer (fact_value f) = party_buyer (fact_value b)
+  \<and> party_broker (fact_value f) = party_broker (fact_value b) #}"
+
 definition "offers_for_budget s b =
-  {# f \<in># facts_of_type Offer s. Offer_buyer f = Budget_buyer b \<and> Offer_broker f = Budget_broker b #}"
+  {# f \<in># facts_of_type Offer s.
+    party_buyer (fact_value f) = party_buyer (fact_value b)
+  \<and> party_broker (fact_value f) = party_broker (fact_value b) #}"
 
 definition "budget_matches_order b order =
-  (Order_buyer order = Budget_buyer b \<and> Order_broker order = Budget_broker b)"
+  (party_buyer (fact_value order) = party_buyer (fact_value b)
+ \<and> party_broker (fact_value order) = party_broker (fact_value b))"
 (* TODO: Budget is missing the description, so we only allow one order per buyer.
    We should add the restriction that budgets are specific to order descriptions *)
 
@@ -242,24 +218,27 @@ definition "budgets_for_order s order =
 
 (* Invariant: a Budget is OK if the sum of its bids and invoices are less than the budget.
    The remaining must be the budget minus whatever has been committed in bids and invoices. *)
-definition budget_ok :: "store \<Rightarrow> fact \<Rightarrow> bool" where
+definition budget_ok :: "Value store \<Rightarrow> Value fact \<Rightarrow> bool" where
 "budget_ok s b = 
     (let bids        = bids_for_budget s b
   in let invoices    = invoices_for_budget s b
   in let offers      = offers_for_budget s b
-  in let sum_all = sum_mset (image_mset Bid_price      bids)
-                 + sum_mset (image_mset Invoice_amount invoices)
-                 + sum_mset (image_mset Offer_price    offers)
-  in sum_all \<le> Budget_budget b \<and> Budget_remain b = Budget_budget b - sum_all)"
+  in let sum_all = sum_mset (image_mset (price_amount o fact_value) bids)
+                 + sum_mset (image_mset (price_amount o fact_value) invoices)
+                 + sum_mset (image_mset (price_amount o fact_value) offers)
+  in sum_all \<le> budget_total (fact_value b)
+  \<and> budget_remain (fact_value b) = budget_total (fact_value b) - sum_all)"
 
 (* Invariant: an Order is OK if all the budgets (there should only be one) are OK *)
-definition order_ok :: "store \<Rightarrow> fact \<Rightarrow> bool" where
+definition order_ok :: "Value store \<Rightarrow> Value fact \<Rightarrow> bool" where
 "order_ok s order = 
   ((size (budgets_for_order s order) \<le> 1) \<and>
-  (\<forall> b \<in># budgets_for_order s order. budget_ok s b \<and> Budget_budget b = Order_budget order))"
+  (\<forall> b \<in># budgets_for_order s order.
+    budget_ok s b
+  \<and> budget_total (fact_value b) = budget_total (fact_value order)))"
 
 (* Invariant: a store is OK if all the orders are OK *)
-definition store_ok :: "store \<Rightarrow> bool" where
+definition store_ok :: "Value store \<Rightarrow> bool" where
 "store_ok s = 
   (\<forall> order \<in># facts_of_type Order s. order_ok s order)"
 
@@ -323,303 +302,82 @@ lemma store_ok__add_order:
   using multi_member_split apply force
   by (simp add: Bid_def Invoice_def Offer_def budget_ok__add_irrelevant_fact)
 
+
 (* The broker can add a new budget for which there are no pre-existing bids or invoices *)
 lemma store_ok__add_budget:
     "store_ok s
  \<Longrightarrow> fact_name b = Budget
- \<Longrightarrow> Budget_remain b = Budget_budget b
+ \<Longrightarrow> budget_remain (fact_value b) = budget_total (fact_value b)
  \<Longrightarrow> bids_for_budget s b = {#}
  \<Longrightarrow> invoices_for_budget s b = {#}
  \<Longrightarrow> offers_for_budget s b = {#}
- \<Longrightarrow> (\<forall>or \<in># facts_of_type Order s. budget_matches_order b or \<longrightarrow> budgets_for_order s or = {#} \<and> Order_budget or = Budget_budget b)
+ \<Longrightarrow> (\<forall>or \<in># facts_of_type Order s. budget_matches_order b or \<longrightarrow> budgets_for_order s or = {#} \<and> budget_total (fact_value or) = budget_total (fact_value b))
  \<Longrightarrow> store_ok ({#b#} \<union># s)"
   unfolding store_ok_def order_ok_def budget_ok_def
     facts_of_type_def bids_for_budget_def invoices_for_budget_def offers_for_budget_def 
-    Invoice_def Bid_def Budget_def
-    store_ok_def order_ok_def
-    budget_matches_order_def
-    budgets_for_order_def facts_of_type_def
-    Budget_def Order_def Offer_def
+    budget_matches_order_def budgets_for_order_def facts_of_type_def
+    Invoice_def Bid_def Budget_def Budget_def Order_def Offer_def
   apply simp
   apply (intro allI conjI impI)
   by (metis (no_types, lifting))+
 
 
-lemma budget_ok__bid_to_offer:
-"budget_ok (add_mset fb s) b \<Longrightarrow>
-       fact_name fb = Bid \<Longrightarrow>
-       fact_name fo = Offer \<Longrightarrow>
-       Offer_lot fo = Bid_lot fb \<Longrightarrow>
-       Offer_broker fo = Bid_broker fb \<Longrightarrow>
-       Offer_buyer fo = Bid_buyer fb \<Longrightarrow>
-       Offer_price fo = Bid_price fb \<Longrightarrow>
-       budget_ok
-        (add_mset
-          fo
-          s) b"
+lemma store_ok__add_budget:
+  "store_ok (add_mset fb s) \<Longrightarrow>
+   fc \<in># s \<Longrightarrow>
+   fact_name fb = Bid \<Longrightarrow>
+   fact_name fc = Item \<Longrightarrow>
+   item_lot (fact_value fc) = item_lot (fact_value fb) \<Longrightarrow>
+   price_amount (fact_value fb) \<le> price_amount (fact_value fc) \<Longrightarrow>
+   store_ok
+    (add_mset
+      (mk_Offer (item_lot (fact_value fb)) (party_broker (fact_value fb)) (party_buyer (fact_value fb)) (price_amount (fact_value fb)) by obs)
+      s)"
+  unfolding store_ok_def order_ok_def budget_ok_def
+    Invoice_def Bid_def Budget_def Budget_def Order_def Offer_def
+  apply simp
   unfolding store_ok_def order_ok_def budget_ok_def
     facts_of_type_def bids_for_budget_def invoices_for_budget_def offers_for_budget_def 
-    Invoice_def Bid_def Budget_def
-    store_ok_def order_ok_def
-    budget_matches_order_def
-    budgets_for_order_def facts_of_type_def
-    Budget_def Order_def Offer_def
-  apply simp
-  apply (intro allI conjI impI)
-   apply (elim conjE)
-   apply (smt ab_semigroup_add_class.add_ac(1) add.commute sum_mset.insert)
-  by auto
+    budget_matches_order_def budgets_for_order_def facts_of_type_def
+    Invoice_def Bid_def Budget_def Budget_def Order_def Offer_def
+    mk_Invoice_def mk_Bid_def mk_Budget_def mk_Budget_def mk_Order_def mk_Offer_def
 
-lemma store_ok__bid_to_offer:
-"store_ok (add_mset fb s) \<Longrightarrow>
-       fact_name fb = Bid \<Longrightarrow>
-       fact_name fo = Offer \<Longrightarrow>
-       Offer_lot fo = Bid_lot fb \<Longrightarrow>
-       Offer_broker fo = Bid_broker fb \<Longrightarrow>
-       Offer_buyer fo = Bid_buyer fb \<Longrightarrow>
-       Offer_price fo = Bid_price fb \<Longrightarrow>
-       store_ok
-        (add_mset
-          fo
-          s)"
-  unfolding store_ok_def order_ok_def
-    facts_of_type_def bids_for_budget_def invoices_for_budget_def offers_for_budget_def 
-    Invoice_def Bid_def Budget_def
-    store_ok_def order_ok_def
-    budget_matches_order_def
-    budgets_for_order_def facts_of_type_def
-    Budget_def Order_def Offer_def
+  apply (simp only: Multiset.set_mset_filter
+                    Multiset.sup_union_left1
+                    Multiset.filter_mset_add_mset
+                    Multiset.set_mset_sup
+                    Set.mem_Collect_eq Set.ball_simps
+                    Multiset.filter_sup_mset
+                    HOL.conj_assoc
+                    fact.simps Cancellation.iterate_add_distrib Multiset.repeat_mset_iterate_add Multiset.add_mset_replicate_mset_safe
+                    fact_ctor.inject list.inject char.inject HOL.simp_thms if_False if_True
+                     Set.Ball_def)
+  apply (intro allI)
+  apply (erule_tac x="x" in allE)
   apply simp
-  apply (intro allI conjI impI)
-  apply (elim conjE)
-  using Bid_def Offer_def budget_ok__bid_to_offer by fastforce
+  apply (intro allI conjI impI; simp)
+   apply (elim allE conjE impE; blast?)
+   apply (simp add: add.assoc add.left_commute)
+  apply (elim allE conjE impE; blast?)
+  oops
 
-lemma store_ok__bid_to_offer__mk_Offer:
-"store_ok (add_mset fb s) \<Longrightarrow>
-       fact_name fb = Bid \<Longrightarrow>
-       store_ok
-        (add_mset
-          (mk_Offer (Bid_lot fb) (Bid_broker fb) (Bid_buyer fb) (Bid_price fb) by obs)
-          s)"
-  unfolding  
-    mk_Offer_def mk_OfferPayload_def mk_BidPayload_def
-    Offer_price_def Bid_price_def
-    Offer_buyer_def Bid_buyer_def
-    Offer_broker_def Bid_broker_def
-  apply simp
-  apply (rule store_ok__bid_to_offer; assumption?; simp?)
-  apply (simp add: Offer_lot_def Bid_lot_def)
-    apply (simp add: Offer_broker_def Bid_broker_def)
-    apply (simp add: Offer_buyer_def Bid_buyer_def)
-    apply (simp add: Offer_price_def Bid_price_def)
-  done
 
-lemma store_ok__bid_to_offer__mk_Offer_rm:
-"store_ok s \<Longrightarrow>
-       fb \<in># s \<Longrightarrow>
-       fact_name fb = Bid \<Longrightarrow>
-       store_ok
-        (add_mset
-          (mk_Offer (Bid_lot fb) (Bid_broker fb) (Bid_buyer fb) (Bid_price fb) by obs)
-          (s - {#fb#}))"
-  using store_ok__bid_to_offer__mk_Offer by fastforce
 
 lemma store_ok__auction_bid__ok:
     "store_ok s
  \<Longrightarrow> asub | s \<turnstile> auction_bid \<Down> fread | dspent | dnew | s' FIRE
  \<Longrightarrow> store_ok s'"
-  unfolding auction_bid_def
-    item_v_def accept_v_def bid_v_def
-    match_any_def match_any_when_def match_first_when_def
-  apply (elim EvFire.cases EvExec.cases; clarsimp)
-  apply (erule EvMatches.cases; clarsimp; erule EvMatches.cases; clarsimp; erule EvMatches.cases; clarsimp)
-  apply (elim EvMatch.cases)
-  apply (elim EvGather.cases)
-  apply (elim EvGain.cases; clarsimp; elim EvSelect.cases; clarsimp; elim EvConsume.cases; clarsimp)
-  apply (unfold check_gather_def)
-  apply clarsimp
-  using store_ok__bid_to_offer__mk_Offer_rm by fastforce
-
-lemma store_ok__accept_offer_ok:
-      "store_ok ({#fe, fd, fc#} + s) \<Longrightarrow>
-       fact_name fc = Accept \<Longrightarrow>
-       fact_name fd = Offer \<Longrightarrow>
-       fact_name fe = Item \<Longrightarrow>
-       Accept_lot fc = Item_lot fe \<Longrightarrow>
-       Offer_lot fd = Item_lot fe \<Longrightarrow>
-       Offer_broker fd = Accept_broker fc \<Longrightarrow>
-       store_ok
-        (add_mset
-          (mk_Invoice (Accept_broker fc) (Offer_buyer fd) (Item_desc fe) (Offer_price fd) by obs)
-          s)"
-  unfolding store_ok_def order_ok_def budget_ok_def
-    facts_of_type_def bids_for_budget_def invoices_for_budget_def offers_for_budget_def 
-    Invoice_def Bid_def Budget_def
-    store_ok_def order_ok_def
-    budget_matches_order_def
-    budgets_for_order_def facts_of_type_def
-    Budget_def Order_def Offer_def Item_def Accept_def
-    mk_Invoice_def
-  apply (simp only: Multiset.set_mset_filter
-                    Multiset.sup_union_left1
-                    Multiset.filter_mset_add_mset
-                    Multiset.set_mset_sup
-                    Set.mem_Collect_eq
-                    Multiset.filter_sup_mset
-                    HOL.conj_assoc
-                    fact.simps
-                    fact_ctor.inject list.inject char.inject HOL.simp_thms if_False if_True)
-  apply simp
-  apply (simp add: Invoice_amount_def Invoice_buyer_def Invoice_broker_def mk_InvoicePayload_def)
-  apply (intro allI conjI impI)
-   apply clarsimp
-   apply (elim allE conjE impE)
-     apply blast
-    apply blast
-   apply (simp add: add.assoc add.left_commute)
-  apply clarsimp
-  apply (erule allE)
-  apply (case_tac "Offer_buyer fd = Budget_buyer b"; clarsimp)
-  apply (elim allE conjE impE)
-       apply blast
-      apply blast
-   apply simp
-  apply (elim allE conjE impE)
-    apply blast
-   apply blast
-  apply simp
-  done
+  oops
 
 lemma store_ok__auction_accept__ok:
     "store_ok s
  \<Longrightarrow> asub | s \<turnstile> auction_accept \<Down> fread | dspent | dnew | s' FIRE
  \<Longrightarrow> store_ok s'"
-  unfolding auction_accept_def
-    item_v_def accept_v_def bid_v_def offer_v_def
-    match_any_def match_any_when_def match_first_when_def
-  apply (elim EvFire.cases EvExec.cases; clarsimp)
-  apply (erule EvMatches.cases; clarsimp)+
-  apply (elim EvMatch.cases)
-  apply (elim EvGather.cases)
-  apply clarsimp
-  apply (elim EvGain.cases; clarsimp)
-  apply (elim EvSelect.cases; clarsimp)
-  apply (elim EvConsume.cases; clarsimp)
-  apply (unfold check_gather_def)
-  apply clarsimp
-  using store_ok__accept_offer_ok
-  by (smt Accept_def Invoice_def Item_def Offer_def char.inject diff_add_mset_swap fact_ctor.inject insert_iff list.inject mk_Invoice_def select_convs(1) set_mset_add_mset_insert set_mset_empty singletonD subset_mset.add_diff_inverse)
-
-
-
-lemma store_ok__add_bid_budget_ok:
-"store_ok ({#fc, fb#} + s) \<Longrightarrow>
-       fa \<in># s \<Longrightarrow>
-       f \<in># s \<Longrightarrow>
-       fact_name fa = Item \<Longrightarrow>
-       Item_desc fa = Order_desc f \<Longrightarrow>
-       fact_name f = Order \<Longrightarrow>
-       fact_name fb = Reserve \<Longrightarrow>
-       fact_name fc = Budget \<Longrightarrow>
-       Reserve_broker fb = Budget_broker fc \<Longrightarrow>
-       Order_broker f = Budget_broker fc \<Longrightarrow>
-       Reserve_buyer fb = Budget_buyer fc \<Longrightarrow>
-       Order_buyer f = Budget_buyer fc \<Longrightarrow>
-       Reserve_amount fb \<le> Budget_remain fc \<Longrightarrow>
-       Reserve_lot fb = Item_lot fa \<Longrightarrow>
-       Reserve_amount fb \<le> Order_limit f \<Longrightarrow>
-       store_ok
-        (add_mset
-          (mk_Budget (Budget_broker fc) (Budget_buyer fc) (Budget_budget fc) (Budget_remain fc - Reserve_amount fb)
-            buby buobs)
-          (add_mset
-            (mk_Bid (Item_lot fa) (Budget_broker fc) (Budget_buyer fc) (Reserve_amount fb)
-              biby biobs)
-            s))"
-  unfolding store_ok_def order_ok_def budget_ok_def
-    facts_of_type_def bids_for_budget_def invoices_for_budget_def offers_for_budget_def 
-    Invoice_def Bid_def Budget_def
-    store_ok_def order_ok_def
-    budget_matches_order_def
-    budgets_for_order_def facts_of_type_def
-    Budget_def Order_def Offer_def Item_def Accept_def Reserve_def
-    mk_Bid_def mk_BidPayload_def mk_Budget_def mk_BudgetPayload_def
-  apply (simp only: Multiset.set_mset_filter
-                    Multiset.sup_union_left1
-                    Multiset.filter_mset_add_mset
-                    Multiset.set_mset_sup
-                    Set.mem_Collect_eq
-                    Multiset.filter_sup_mset
-                    HOL.conj_assoc
-                    fact.simps
-                    fact_ctor.inject list.inject char.inject HOL.simp_thms if_False if_True
-                    Set.ball_simps)
-  apply simp
-  apply (simp add: Bid_buyer_def Budget_buyer_def Bid_broker_def Budget_broker_def
-      Bid_price_def Budget_budget_def Budget_remain_def
-      Invoice_amount_def Invoice_buyer_def Invoice_broker_def mk_InvoicePayload_def)
-  apply (intro allI impI)
-  apply (intro allI conjI impI)
-   apply (elim allE conjE impE)
-     apply blast
-        apply blast
-  apply (simp add: Bid_buyer_def Budget_buyer_def Bid_broker_def Budget_broker_def
-      Bid_price_def Budget_budget_def Budget_remain_def
-      Invoice_amount_def Invoice_buyer_def Invoice_broker_def mk_InvoicePayload_def)
-
-
-   apply (elim allE conjE impE; blast?)
-  apply (smt Nat.le_diff_conv2 ab_semigroup_add_class.add_ac(1) diff_cancel2 le_add_diff_inverse2)
-
-     apply (elim allE conjE impE; blast?)
-  apply (simp add: Bid_buyer_def Budget_buyer_def Bid_broker_def Budget_broker_def
-      Bid_price_def Budget_budget_def Budget_remain_def
-      Invoice_amount_def Invoice_buyer_def Invoice_broker_def mk_InvoicePayload_def)
-  using multi_member_split apply force
-
-     apply (erule_tac x="order" in allE)
-    apply (case_tac "Order_buyer order = fst (snd (tk_BudgetPayload (fact_value fc)))"; clarsimp)
-     apply (simp add: Bid_buyer_def Budget_buyer_def Bid_broker_def Budget_broker_def Bid_price_def Budget_budget_def Budget_remain_def)
-     apply (simp add: Bid_buyer_def Budget_buyer_def Bid_broker_def Budget_broker_def Bid_price_def Budget_budget_def Budget_remain_def)
-
-   apply (elim allE conjE impE; blast?; simp)
-    apply simp
-  by blast
-
+  oops
 
 lemma store_ok__broker_reserve__ok:
     "store_ok s
  \<Longrightarrow> asub | s \<turnstile> broker_reserve \<Down> fread | dspent | dnew | s' FIRE
  \<Longrightarrow> store_ok s'"
-  unfolding broker_reserve_def
-    item_v_def accept_v_def bid_v_def offer_v_def budget_v_def reserve_v_def order_v_def
-    match_any_def match_any_when_def match_first_when_def
-  apply (elim EvFire.cases EvExec.cases; clarsimp)
-  apply (erule EvMatches.cases; clarsimp)+
-  apply (elim EvMatch.cases)
-  apply (elim EvGather.cases)
-  apply clarsimp
-  apply (elim EvGain.cases; clarsimp)
-  apply (elim EvSelect.cases; clarsimp)
-  apply (elim EvConsume.cases; clarsimp)
-  apply (unfold check_gather_def)
-
-  apply (rule_tac V="store_ok
-        (add_mset
-          (mk_Budget (Budget_broker fc) (Budget_buyer fc) (Budget_budget fc) (Budget_remain fc - Reserve_amount fb)
-            {Budget_broker fc} {})
-          (add_mset
-            (mk_Bid (Item_lot fa) (Reserve_broker fb) (Order_buyer f) (Reserve_amount fb) {Reserve_broker fb, Order_buyer f}
-              {party ''Mark''})
-            (s -
-         {#fc, fb#})))" in revcut_rl)
-
-   apply clarsimp
-   apply (rule store_ok__add_bid_budget_ok; blast?; simp add: find_firsts_def)
-  apply (metis (no_types, lifting) add_mset_remove_trivial mset_subset_eq_single subset_mset.add_diff_assoc2 subset_mset.add_diff_inverse union_single_eq_member)
-    apply (smt Budget_def Item_def Reserve_def char.inject fact_ctor.inject insert_iff list.inject set_mset_add_mset_insert set_mset_empty singletonD subset_mset.add_diff_inverse union_iff)
-  defer
-  apply (smt add_mset_commute add_mset_diff_bothsides add_mset_remove_trivial add_mset_remove_trivial_If diff_union_swap insert_subset_eq_iff)
-  by (smt Budget_def Multiset.diff_cancel Order_def Reserve_def add_mset_remove_trivial char.inject fact_ctor.inject insert_DiffM insert_noteq_member list.inject mset_subset_eq_add_mset_cancel subset_mset.add_diff_assoc2 subset_mset.add_diff_inverse subset_mset.sup.orderI subset_mset.sup_bot.right_neutral)
-
+  oops
 end
