proof/Exp.thy
@@ -6,28 +6,30 @@ begin
 
 (* As the term language is standard, we use a HOAS representation with a heap that maps variable names to facts *)
 datatype     fact_var = fact_var string
-type_synonym fact_env = "fact_var \<Rightarrow> fact"
-type_synonym 'a exp   = "fact_env \<Rightarrow> 'a"
+(* The fact heap is parameterised by the type of fact payloads. *)
+type_synonym 'f fact_env = "fact_var \<Rightarrow> 'f fact"
+(* Expressions are parameterised by the type of fact payloads and result type. *)
+type_synonym ('f,'r) exp   = "'f fact_env \<Rightarrow> 'r"
 
 (* Matches: there are four parts to a match: gather, select, consume, and gain. *)
 
 (* Gather: filter input facts according to constructor name and a boolean expression.
    In the paper, this is a list of expressions, but here we just join multiple expressions with conjunction *)
-datatype gather = gather_when fact_ctor "bool exp"
+datatype 'f gather = gather_when fact_ctor "('f,bool) exp"
 
 (* Select: gathering can return many input facts, and select specifies which of these facts to choose *)
-datatype select = select_any | select_first "nat exp"
+datatype 'f select = select_any | select_first "('f,nat) exp"
 
 (* Consume: how many instances of a certain fact do we need? *)
-datatype consume = consume_weight "nat exp"
+datatype 'f consume = consume_weight "('f,nat) exp"
 
 (* Gain: extract authority from a fact *)
-datatype gain = gain_auth "auth exp"
+datatype 'f gain = gain_auth "('f,auth) exp"
 
 (* Match puts these four components together, along with a name to bind the fact *)
-datatype match = match fact_var gather select consume gain
+datatype 'f match = match fact_var "'f gather" "'f select" "'f consume" "'f gain"
 
 (* A rule has a rule name, a list of matches, and a 'say' expression to return the new facts *)
-datatype rule = rule rule_name "match list" "store exp"
+datatype 'f rule = rule rule_name "'f match list" "('f, 'f store) exp"
 
 end
